Just before meeting

theories/Iris/BinaryAdequacy.v
@@ -226,6 +226,25 @@ Module Type IrisAdequacy2
     induction 1; econstructor; eassumption.
   Qed.
 
+  Inductive NStepsWithExitCond {Γ : PCtx} (exitCond : RegStore -> Memory -> Prop) {σ : Ty} (γ1 : RegStore) (μ1 : Memory) (δ1 : CStoreVal Γ) (s1 : Stm Γ σ) : RegStore -> Memory -> CStoreVal Γ -> Stm Γ σ -> nat -> Prop :=
+  | nstepWithExitCond_refl : NStepsWithExitCond exitCond γ1 μ1 δ1 s1 γ1 μ1 δ1 s1 0
+  | nstepWithExitCond_trans {n} {γ2 γ3 : RegStore} {μ2 μ3 : Memory} {δ2 δ3 : CStoreVal Γ} {s2 s3 : Stm Γ σ} :
+    ~ exitCond γ1 μ1 -> Step γ1 μ1 δ1 γ2 μ2 δ2 s1 s2 -> NStepsWithExitCond exitCond γ2 μ2 δ2 s2 γ3 μ3 δ3 s3 n -> NStepsWithExitCond exitCond γ1 μ1 δ1 s1 γ3 μ3 δ3 s3 (S n).
+
+  Lemma stepsWithExitCond_to_nstepsWithExitCond {Γ : PCtx} exitCond {σ : Ty} {γ1 γ2 : RegStore} {μ1 μ2 : Memory} {δ1 δ2 : CStoreVal Γ} {s1 s2 : Stm Γ σ} :
+    StepsWithExitCond exitCond γ1 μ1 δ1 s1 γ2 μ2 δ2 s2 -> exists n, NStepsWithExitCond exitCond γ1 μ1 δ1 s1 γ2 μ2 δ2 s2 n.
+  Proof.
+    induction 1 as [|γ1 μ1 δ1 s1 γ2 γ3 μ2 μ3 δ2 δ3 s2 s3 notEC eval evals [n nsteps]].
+    - exists 0. constructor.
+    - exists (S n). econstructor; eassumption.
+  Qed.
+
+  Lemma nstepsWithExitCond_to_stepsWithExitCond {Γ : PCtx} exitCond {σ : Ty} {γ1 γ2 : RegStore} {μ1 μ2 : Memory} {δ1 δ2 : CStoreVal Γ} {s1 s2 : Stm Γ σ} {n} :
+    NStepsWithExitCond exitCond γ1 μ1 δ1 s1 γ2 μ2 δ2 s2 n -> StepsWithExitCond exitCond γ1 μ1 δ1 s1 γ2 μ2 δ2 s2.
+  Proof.
+    induction 1; econstructor; eassumption.
+  Qed.
+
   (* TODO: move following 3 to where stm_val_stuck is defined? *)
   Lemma final_val_and_fail_None : forall {Γ τ} (s : Stm Γ τ),
       Final s -> stm_to_val s = None -> stm_to_fail s = None -> False.
@@ -433,6 +452,70 @@ Module Type IrisAdequacy2
       now iMod (IHHevaln1 with "[$Hmem $Hregs $Hwp2 $Hinv] Hcredn") as "IH".
   Qed.
 
+    Lemma adequacy_gen_withExitCond {Γ σ} exitCond (s11 s21 : Stm Γ σ) {γ11 γ12 γ21} {μ11 μ12 μ21}
+    {δ11 δ12 δ21 : CStoreVal Γ} {s12 : Stm Γ σ} {Q : forall `{sailGS2 Σ}, IVal σ -> CStoreVal Γ -> IVal σ -> CStoreVal Γ -> iProp Σ}
+    (φ : Prop) :
+    ⟨ γ11, μ11, δ11, s11 ⟩ -( exitCond )->* ⟨ γ12, μ12, δ12, s12 ⟩ ->
+    (forall `{sailGS2 Σ},
+        mem_res2 μ11 μ21 ∗ own_regstore2 γ11 γ21 ⊢ |={⊤}=> semWP2 δ11 δ21 s11 s21 Q
+        ∗ (∀ μ22, mem_inv2 μ12 μ22 ={⊤,∅}=∗ ⌜φ⌝)
+    )%I -> φ.
+  Proof.
+    intros Heval1 Hwp.
+    destruct (stepsWithExitCond_to_nstepsWithExitCond Heval1) as [n Hevaln1].
+    refine (uPred.pure_soundness _
+              (step_fupdN_soundness_gen (Σ := sailΣ2) _ HasLc n n _)).
+    iIntros (Hinv) "".
+    iMod (own_alloc ((● RegStore_to_map γ11 ⋅ ◯ RegStore_to_map γ11 ) : regUR)) as (regs1) "[Hregsown1 Hregsinv1]".
+    { apply auth_both_valid.
+      intuition.
+      apply RegStore_to_map_valid. }
+    iMod (own_alloc ((● RegStore_to_map γ21 ⋅ ◯ RegStore_to_map γ21 ) : regUR)) as (regs2) "[Hregsown2 Hregsinv2]".
+    { apply auth_both_valid.
+      intuition.
+      apply RegStore_to_map_valid. }
+    pose proof (memΣ_GpreS2 (Σ := sailΣ2) _) as mGS.
+    iMod (mem_inv_init2 (mGS := mGS) μ11 μ21) as (memG) "[Hmem Rmem]".
+    pose (sG := @SailGS2 sailΣ2 Hinv (SailRegGS2 (SailRegGS reg_pre_inG2_left regs1) (SailRegGS reg_pre_inG2_right regs2)) memG).
+    specialize (Hwp _ sG).
+    iPoseProof (Hwp with "[$Rmem Hregsinv1 Hregsinv2]") as "Hwp2".
+    { iApply own_RegStore_to_map_reg_pointsTos.
+      apply finite.NoDup_enum.
+      iSplitR "Hregsinv2"; iAssumption.
+    }
+    iAssert (regs_inv2 γ11 γ21) with "[Hregsown1 Hregsown2]" as "Hregs".
+    { iSplitL "Hregsown1";
+      now iApply own_RegStore_to_regs_inv.
+    }
+    clear Hwp.
+    iStopProof.
+    revert γ21 μ21 δ21 s21.
+    induction Hevaln1.
+    - iIntros (γ21 μ21 δ21 s21) "(Hmem & Hwp2 & Hregs) Hcred".
+      iMod "Hwp2" as "[_ Hcont]".
+      iMod ("Hcont" with "Hmem") as "%Hφ".
+      cbn. done.
+    - iIntros (γ21 μ21 δ21 s21) "(Hregs & Hwp2 & Hmem) Hcred".
+      specialize (IHHevaln1 (nstepsWithExitCond_to_stepsWithExitCond Hevaln1)).
+      rewrite fixpoint_semWP2_eq; cbn.
+      rewrite (stm_val_stuck H0).
+      repeat case_match;
+        try (iMod "Hwp2" as "(H & _)";
+             by iMod "H").
+      iMod "Hwp2".
+      iDestruct "Hwp2" as "(Hwp2 & Hinv)".
+      iSpecialize ("Hwp2" with "[$Hregs $Hmem]").
+      assert (stm_to_fail s21 = None) as H2.
+      { destruct s21; cbn in *; inversion H1; done. }
+      pose proof (is_not_final s21 H1 H2) as Hnfinal21.
+      destruct (can_step s21 γ21 μ21 δ21 Hnfinal21) as (γ22 & μ22 & δ22 & s22 & Hsteps21).
+      iMod "Hwp2" as "Hwp2". iModIntro.
+      iSpecialize ("Hwp2" $! _ _ _ _ _ _ _ _ (conj H0 Hsteps21)).
+      iMod "Hwp2". iModIntro. iModIntro. iMod "Hwp2".
+      iDestruct "Hcred" as "(Hcred1 & Hcredn)".
+      iMod "Hwp2" as "([Hregs Hmem] & Hwp2)".
+      now iMod (IHHevaln1 with "[$Hmem $Hregs $Hwp2 $Hinv] Hcredn") as "IH".
+  Qed.
 
   (* Lemma wp2_adequacy' {Γ1 Γ2 τ} (s1 : Stm Γ1 τ) (s2 : Stm Γ2 τ) *)
   (*   {γ1 γ2 : RegStore} {μ1 μ2 : Memory} *)
